interface for Cert

src/tls/Cert.fst
@@ -9,38 +9,6 @@ open TLSConstants
 open Extensions // defining cert, cert13, chain
 open Parse
  
-(* The chain format changes between TLS 1.2 and TLS 1.3; we separate
-then in messages, but at least for now, we merge the two in
-Negotiation and in the main TLS API (with no extensions when using TLS
-1.2 *)
-
-// opaque cert_data<1..2^24-1>
-type cert = b:bytes {length b < 16777216}
-type certes = cert * (exts:extensions{length (extensionListBytes exts) < 65536 /\ bindersLen exts == 0})
-// CertificateEntry certificate_list<0..2^24-1>;
-// See https://tlswg.github.io/tls13-spec/#rfc.section.4.4.2
-type chain = l:list cert // { ... }
-type chain13 = l:list certes // { ... }
-
-// we may use these types to keep track of un-extended chains,
-// e.g. to prove that their formatting is injective
-let is_classic_chain_aux (ces:certes) = List.Tot.isEmpty (snd ces)
-let is_classic_chain (l:chain13): bool =
-  List.Tot.for_all #certes is_classic_chain_aux l
-type chain12 = l:chain13 {is_classic_chain l}
-
-// 2018.03.10 SZ: The types in Extensions.fsti are too weak to prove the refinement in [certes]
-#set-options "--admit_smt_queries true"
-// todo: prove it is a chain12
-let chain_up_aux (c:cert) : certes = c, []
-#reset-options
-
-let chain_up (l:chain): chain13= List.Tot.map #cert #certes chain_up_aux l
-let chain_down (l:chain13): chain = List.Tot.map #certes #cert fst l
-
-(* ------------------------------------------------------------------------ *)
-
-abstract val certificateListBytes: chain -> Tot bytes
 let rec certificateListBytes = function
   | [] -> empty_bytes
   | crt :: rest ->
@@ -49,7 +17,6 @@ let rec certificateListBytes = function
     assume (UInt.size (3 + length crt + length (certificateListBytes rest)) UInt32.n);
     vlbytes 3 crt @| certificateListBytes rest
 
-abstract val certificateListBytes13: chain13 -> Tot bytes
 let rec certificateListBytes13 = function
   | [] -> empty_bytes
   | (crt, exts) :: rest ->
@@ -58,51 +25,6 @@ let rec certificateListBytes13 = function
     assume (UInt.size (3 + length crt + length (extensionsBytes exts) + length (certificateListBytes13 rest)) UInt32.n);
     vlbytes 3 crt @| extensionsBytes exts @| certificateListBytes13 rest
 
-val certificateListBytes_is_injective: c1:chain -> c2:chain ->
-  Lemma (Bytes.equal (certificateListBytes c1) (certificateListBytes c2) ==> c1 == c2)
-
-#set-options "--admit_smt_queries true"
-// 2018.03.10: Lax-typecheck for now; this will be reimplemented in LowParse anyway
-let rec certificateListBytes_is_injective c1 c2 =
-  match c1, c2 with
-  | [], [] -> ()
-  | hd::tl, hd'::tl' ->
-    if certificateListBytes c1 = certificateListBytes c2 then
-      begin
-      lemma_repr_bytes_values (length hd); lemma_repr_bytes_values (length hd');
-      cut(Bytes.equal ((vlbytes 3 hd) @| (certificateListBytes tl)) ((vlbytes 3 hd') @| (certificateListBytes tl')));
-      lemma_repr_bytes_values (length hd);
-      lemma_repr_bytes_values (length hd');
-      cut(Bytes.equal (Bytes.slice (vlbytes 3 hd) 0ul 3ul) (Bytes.slice (certificateListBytes c1) 0ul 3ul));
-      cut(Bytes.equal (Bytes.slice (vlbytes 3 hd') 0ul 3ul) (Bytes.slice (certificateListBytes c1) 0ul 3ul));
-      vlbytes_length_lemma 3 hd hd';
-      //lemma_append_inj (vlbytes 3 hd) (certificateListBytes tl) (vlbytes 3 hd') (certificateListBytes tl'); //TODO bytes NS 09/27
-      lemma_vlbytes_inj 3 hd hd';
-      certificateListBytes_is_injective tl tl'
-      end
-  | [], hd::tl ->
-    begin
-    cut (length (certificateListBytes c1) = 0);
-    lemma_repr_bytes_values (length hd);
-    cut (Bytes.equal (certificateListBytes c2) ((vlbytes 3 hd) @| (certificateListBytes tl)));
-    lemma_vlbytes_len 3 hd
-    end
-  | hd::tl, [] ->
-    begin
-    cut (length (certificateListBytes c2) = 0);
-    lemma_repr_bytes_values (length hd);
-    cut (Bytes.equal (certificateListBytes c1) ((vlbytes 3 hd) @| (certificateListBytes tl)));
-    lemma_vlbytes_len 3 hd
-    end
-#reset-options
-
-val certificateListBytes13_is_injective: c1:chain13 -> c2:chain13 ->
-  Lemma (Bytes.equal (certificateListBytes13 c1) (certificateListBytes13 c2) ==> c1 == c2)
-let rec certificateListBytes13_is_injective c1 c2 =
-  // TODO: need injectivity lemmas for extensions
-  admit()
-
-abstract val parseCertificateList: b:bytes -> Tot (result chain) (decreases (length b))
 let rec parseCertificateList b =
   if length b = 0 then Correct [] else
   
@@ -116,7 +38,6 @@ let rec parseCertificateList b =
     | Correct cs -> lemma_repr_bytes_values (length c); Correct (c::cs) )
 
 #set-options "--z3rlimit 50" 
-abstract val parseCertificateList13: b:bytes -> Tot (result chain13) (decreases (length b))
 let rec parseCertificateList13 b =
   if length b = 0 then Correct [] else
   if length b < 3 then fatal Bad_certificate "not enough bytes (certificate length)" else
@@ -145,11 +66,6 @@ let rec parseCertificateList13 b =
 
 #set-options "--z3rlimit 100 --max_ifuel 4"
 
-val lemma_parseCertificateList_length: b:bytes ->
-  Lemma (ensures (match parseCertificateList b with
-      | Correct ces -> length (certificateListBytes ces) == length b
-      | _ -> True))
-  (decreases (length b))
 let rec lemma_parseCertificateList_length b =
   if length b < 3 then ()
   else
