src/tls/Cert.fsti
@@ -1,0 +1,96 @@
+(* Copyright (C) 2012--2018 Microsoft Research and INRIA *)
+module Cert
+
+open FStar.Bytes
+open FStar.Error
+
+open TLSError
+open TLSConstants
+open Extensions // defining cert, cert13, chain
+open Parse
+ 
+(* The chain format changes between TLS 1.2 and TLS 1.3; we separate
+then in messages, but at least for now, we merge the two in
+Negotiation and in the main TLS API (with no extensions when using TLS
+1.2 *)
+
+// opaque cert_data<1..2^24-1>
+type cert = b:bytes {length b < 16777216}
+type certes = cert * (exts:extensions{length (extensionListBytes exts) < 65536 /\ bindersLen exts == 0})
+// CertificateEntry certificate_list<0..2^24-1>;
+// See https://tlswg.github.io/tls13-spec/#rfc.section.4.4.2
+type chain = l:list cert // { ... }
+type chain13 = l:list certes // { ... }
+
+// we may use these types to keep track of un-extended chains,
+// e.g. to prove that their formatting is injective
+let is_classic_chain_aux (ces:certes) = List.Tot.isEmpty (snd ces)
+let is_classic_chain (l:chain13): bool =
+  List.Tot.for_all #certes is_classic_chain_aux l
+type chain12 = l:chain13 {is_classic_chain l}
+
+// 2018.03.10 SZ: The types in Extensions.fsti are too weak to prove the refinement in [certes]
+#set-options "--admit_smt_queries true"
+// todo: prove it is a chain12
+let chain_up_aux (c:cert) : certes = c, []
+#reset-options
+
+let chain_up (l:chain): chain13= List.Tot.map #cert #certes chain_up_aux l
+let chain_down (l:chain13): chain = List.Tot.map #certes #cert fst l
+
+(* ------------------------------------------------------------------------ *)
+
+val certificateListBytes: chain -> Tot bytes
+
+val certificateListBytes13: chain13 -> Tot bytes
+
+#push-options "--admit_smt_queries true"
+let rec certificateListBytes_is_injective: c1:chain -> c2:chain ->
+  Lemma (Bytes.equal (certificateListBytes c1) (certificateListBytes c2) ==> c1 == c2) =
+
+// 2018.03.10: Lax-typecheck for now; this will be reimplemented in LowParse anyway
+  fun c1 c2 -> admit ()  //AR: 04/08: this lemma is anyway admitted, commenting the body below
+  // match c1, c2 with
+  // | [], [] -> ()
+  // | hd::tl, hd'::tl' ->
+  //   if certificateListBytes c1 = certificateListBytes c2 then
+  //     begin
+  //     lemma_repr_bytes_values (length hd); lemma_repr_bytes_values (length hd');
+  //     cut(Bytes.equal ((vlbytes 3 hd) @| (certificateListBytes tl)) ((vlbytes 3 hd') @| (certificateListBytes tl')));
+  //     lemma_repr_bytes_values (length hd);
+  //     lemma_repr_bytes_values (length hd');
+  //     cut(Bytes.equal (Bytes.slice (vlbytes 3 hd) 0ul 3ul) (Bytes.slice (certificateListBytes c1) 0ul 3ul));
+  //     cut(Bytes.equal (Bytes.slice (vlbytes 3 hd') 0ul 3ul) (Bytes.slice (certificateListBytes c1) 0ul 3ul));
+  //     vlbytes_length_lemma 3 hd hd';
+  //     //lemma_append_inj (vlbytes 3 hd) (certificateListBytes tl) (vlbytes 3 hd') (certificateListBytes tl'); //TODO bytes NS 09/27
+  //     lemma_vlbytes_inj 3 hd hd';
+  //     certificateListBytes_is_injective tl tl'
+  //     end
+  // | [], hd::tl ->
+  //   begin
+  //   cut (length (certificateListBytes c1) = 0);
+  //   lemma_repr_bytes_values (length hd);
+  //   cut (Bytes.equal (certificateListBytes c2) ((vlbytes 3 hd) @| (certificateListBytes tl)));
+  //   lemma_vlbytes_len 3 hd
+  //   end
+  // | hd::tl, [] ->
+  //   begin
+  //   cut (length (certificateListBytes c2) = 0);
+  //   lemma_repr_bytes_values (length hd);
+  //   cut (Bytes.equal (certificateListBytes c1) ((vlbytes 3 hd) @| (certificateListBytes tl)));
+  //   lemma_vlbytes_len 3 hd
+  //   end
+#pop-options
+
+let rec certificateListBytes13_is_injective: c1:chain13 -> c2:chain13 ->
+  Lemma (Bytes.equal (certificateListBytes13 c1) (certificateListBytes13 c2) ==> c1 == c2) = fun c1 c2 -> admit ()
+
+val parseCertificateList: b:bytes -> Tot (result chain) (decreases (length b))
+
+val parseCertificateList13: b:bytes -> Tot (result chain13) (decreases (length b))
+
+val lemma_parseCertificateList_length: b:bytes ->
+  Lemma (ensures (match parseCertificateList b with
+      | Correct ces -> length (certificateListBytes ces) == length b
+      | _ -> True))
+  (decreases (length b))
